

# TEST!

Test yourself!

## MAIN MENU

Home

Teaching

Calculus Website

Precalculus Website

Tests

Calculus Tests

Precalculus Tests

Test

Test: Calculus I - Differentiation Formulas - Quiz 1

Number of Questions: 10

Time: 29 : 59

If  $f(x) = \left(\frac{1}{x} + \frac{1}{x^2}\right)(3x^3 + 27)$  then  $f'(x)$  is

$y = 3x^3 + 3x + \frac{27}{x} + \frac{27}{x^2}$

$y' = 6x + 3 - \frac{27}{x^2} - \frac{54}{x^3}$

- ~~$3 + 6x - 27x^{-2} + 54x^{-3}$~~
- ~~$3 + 6x + 27x^{-2} - 54x^{-3}$~~
- ~~$3 - 6x - 27x^{-2} - 54x^{-3}$~~
- ~~$3 + 6x - 27x^{-2} - 54x^{-3}$~~
- $3 + 6x - 27x^{-2} - 54x^{-3}$

If  $y = (2x^7 - x^2)\left(\frac{x-1}{x+1}\right)$  then  $y'(1)$  is

$x^2(2x^5 - x)$

$\frac{2x^8 - 2x^7 - x^3 + x^2}{x+1}$

- 1
- $\frac{1}{3}$
- $\frac{1}{4}$
- $\frac{1}{5}$
- $\frac{1}{2}$

$\rightarrow \frac{(16x^7 - 14x^6 - 3x^2 + 2x) - 2x^8 + 2x^7 + x^3 - x^2}{(x+1)^2}$

$y'(1) = \frac{16 - 14 - 3 + 2 - 2 + 2 + 1 - 1}{4} = \frac{1}{4}$

If  $f(x) = (x^2 + 1)\sec x$  then  $f'(x)$  is  $\frac{x^2+1}{\cos x} \rightarrow \frac{2x\cos x - (x^2+1)(-\sin x)}{\cos^2 x}$

- $-(x^2 + 1)\csc x \tan x + 2\sec x$
- $-(x^2 + 1)\csc x \tan x + 2x\sec x$
- $(x^2 + 1)\csc x \tan x + 2x\sec x$
- $-(x^2 + 1)\sec x \tan x + 2x\sec x$
- $(x^2 + 1)\sec x \tan x + 2x\sec x$

$= 2x\sec x + (x^2+1)\tan x \sec x$

If  $f(x) = \frac{1}{\cot x}$  then  $f'(x)$  is

- $\cot^2 x$
- $\tan^2 x$
- $\cos^2 x$
- $\sin^2 x$
- $\sec^2 x$

$= \tan x \quad d(\tan x) = \sec^2 x$

If  $y = \tan x$  then  $\frac{d^2 y}{dx^2}$  is

- $2 \tan^2 x \sec x$
- $2 \cot^2 x \csc x$
- $2 \sin^2 x \tan x$
- $2 \cos^2 x \cot x$
- $2 \sec^2 x \tan x$

$y' = \sec^2 x$   
 $y'' = 2 \sec x \cdot \sec x \tan x$   
 $= 2 \sec^2 x \tan x$

If  $f(x) = \sin^3 x$  then  $f'(x)$  is

- $-3 \cos^2 x \sin x$
- $3 \sin x \cos x$
- $-3 \sin^2 x \cos x$
- $3 \cos^2 x \sin x$
- $3 \sin^2 x \cos x$

$3 \sin^2 x \cdot \cos x$

If  $f(x) = \cos^3 \left( \frac{x}{x+1} \right)$  then  $f'(x)$  is

- $-\frac{3}{(x+1)^2} \cos^2 \left( \frac{x}{x+1} \right) \sin \left( \frac{x}{x+1} \right)$
- $\frac{3}{(x+1)^2} \cos^2 \left( \frac{x}{x+1} \right) \sin \left( \frac{x}{x+1} \right)$
- $-\frac{3}{(x+1)^2} \cos^2 \left( \frac{x}{x+1} \right)$
- $-\frac{3}{(x+1)^2} \cos^2 \left( \frac{x}{x+1} \right) \cos \left( \frac{x}{x+1} \right)$
- $\frac{3}{(x+1)^2} \cos^2 \left( \frac{x}{x+1} \right)$

$3 \cos^2 \left( \frac{x}{x+1} \right) \cdot \left( -\sin \frac{x}{x+1} \right) d \left( \frac{x}{x+1} \right)$

$= -\frac{3}{(x+1)^2} \cos^2 \frac{x}{x+1} \left( \sin \frac{x}{x+1} \right)$

$\frac{x}{x+1} \rightarrow \frac{x+1-1}{(x+1)^2} = \frac{1}{(x+1)^2}$

$$4x^3 - 8x \sec(4x^2 - 2) \tan(4x^2 - 2)$$

$$(x^3 - 2x \sec \circ \tan)$$

$$4x(x^2 - 2 \sec \circ \tan)$$

If  $f(x) = [x^4 - \sec(4x^2 - 2)]^{-4}$  then  $f'(x)$  is

- $-16x [x^4 - \sec(4x^2 - 2)]^{-5} [x^2 - 2 \cos(4x^2 - 2) \cot(4x^2 - 2)]$
- $-16x [x^4 - \sec(4x^2 - 2)]^{-5} [x^2 - 2 \csc(4x^2 - 2) \cot(4x^2 - 2)]$
- $-16x [x^4 - \sec(4x^2 - 2)]^{-5} [x^2 - 2 \csc(4x^2 - 2) \tan(4x^2 - 2)]$
- $-16x [x^4 - \sec(4x^2 - 2)]^{-5} [x^2 - 2 \sec(4x^2 - 2) \tan(4x^2 - 2)]$
- $-16x [x^4 - \sec(4x^2 - 2)]^{-5} [x^2 - 2 \sec(4x^2 - 2) \cot(4x^2 - 2)]$

If  $y = \frac{\sin x}{\sec(3x + 1)}$  then  $y'$  is

$y = \sin x \cos(3x + 1)$   
 $y = \cos x \cos(3x + 1) + \sin x \sin(3x + 1) \cdot 3$

- None of the above
- $-\cos x \cos(3x + 1) + 3 \sin x \sin(3x + 1)$
- $-\cos x \cos(3x + 1) - 3 \sin x \sin(3x + 1)$
- $\cos x \cos(3x + 1) + 3 \sin x \sin(3x + 1)$
- $\cos x \cos(3x + 1) - 3 \sin x \sin(3x + 1)$

$$\frac{2x(1+x^2) - (1+x^2)(-2x)}{(1-x^2)^2}$$

$$= 2x - 2x + 2x + 2x$$

$$= 4x$$

If  $y = \left(\frac{1+x^2}{1-x^2}\right)^{17}$  then  $y'$  is

$17 \left(\frac{1+x^2}{1-x^2}\right)^{16} \cdot \frac{dy}{dx} \left(\frac{1+x^2}{1-x^2}\right)$

- $\frac{72x(1+x^2)^{16}}{(1-x^2)^{18}}$
  - $\frac{52x(1+x^2)^{16}}{(1-x^2)^{18}}$
  - $\frac{24x(1+x^2)^{16}}{(1-x^2)^{18}}$
  - $\frac{70x(1+x^2)^{16}}{(1-x^2)^{18}}$
  - $\frac{68x(1+x^2)^{16}}{(1-x^2)^{18}}$
- $= 68x \left(\frac{1+x^2}{1-x^2}\right)^{16}$



# TEST!

Test yourself!

## MAIN MENU

- Home
- Teaching
- Calculus Website
- Precalculus Website
- Tests**
- Calculus Tests
- Precalculus Tests

## Test

**Test:** Calculus I - Derivatives of Logarithmic and Exponential Functions - Quiz 1  
**Number of Questions:** 12  
**Time:** 24 : 58

If  $y = \ln\left(\frac{(x^2+1)^5}{\sqrt{1-x}}\right)$ , then  $y'$  is

$$5 \ln x^2 + 1 - \frac{1}{2} \ln(1-x)$$

$$\rightarrow \frac{5 \cdot 2x}{x^2+1} + \frac{1}{2(1-x)} = \frac{10x}{x^2+1} + \frac{1}{2(1-x)}$$

$$d_u = \frac{5 \ln(x^2+1)^4 \cdot (x^2+1)^5 + (x^2+1)^5 \cdot 2 \cdot \sqrt{1-x}}{1-x}$$

$$\sqrt{1-x} \rightarrow -\frac{1}{2\sqrt{1-x}}$$

- $\frac{5x}{x^2+1} + \frac{1}{3(1-x)}$
- $\frac{5x}{x^2+1} + \frac{1}{2(x-1)}$
- $\frac{5x}{x^2+1} + \frac{1}{2(1-x)}$
- $\frac{10x}{x^2+1} + \frac{1}{2(1-x)}$
- $\frac{10x}{x^2+1} + \frac{1}{2(x-1)}$

$$\frac{\sqrt{1-x} \left( \frac{10x(x^2+1)^4}{1-x} + \frac{(x^2+1)^5}{2(1-x)^{1.5}} \right)}{(x^2+1)^5}$$

$$= \frac{10x}{(x^2+1)\sqrt{1-x}} + \frac{1}{2(1-x) \cdot 2(1-x)}$$

$$= \frac{20x}{2(x^2+1)\sqrt{1-x}} + \frac{(x^2+1)\sqrt{1-x}}{2(x^2+1)(1-x)}$$

If  $y = \ln(\ln x)$ , then  $y'$  is

- $\frac{1}{x}$
- $\frac{1}{\ln x}$
- $\frac{\ln x}{x}$
- $\frac{\ln x}{4}$
- $\frac{x \ln x}{1}$
- $\frac{1}{x \ln x}$

$$\frac{1}{\ln x} \cdot \frac{1}{x} = \frac{1}{x \ln x}$$

$x \ln x \rightarrow \ln x + 1$

If  $y = \frac{x \ln x}{1 + \ln x}$ , then  $y'$  is  $\frac{(\ln x + 1)^2 - \ln x}{(1 + \ln x)^2} = \frac{\ln^2 x + 2 \ln x + 1 - \ln x}{(1 + \ln x)^2}$

- $1 - \frac{\ln x}{(1 + \ln x)^2}$
- $\frac{x \ln x}{(1 + \ln x)^2}$
- $1 - \frac{x \ln x}{(1 + \ln x)^2}$
- $1 + \frac{x \ln x}{(1 + \ln x)^2}$
- $1 + \frac{\ln x}{(1 + \ln x)^2}$

If  $y = \frac{1 + \ln t}{t}$ , then  $y'$  is  $\frac{1 - (1 + \ln t)}{t^2} = \frac{-\ln t}{t^2}$

- $-\frac{t + \ln t}{t^2}$
- $-\frac{\ln t}{t^2}$
- $-\frac{2 \ln t}{t^2}$
- $\frac{2 \ln t}{t^2}$
- $\frac{\ln t}{t^2}$

If  $y = t\sqrt{\ln t}$ , then  $y'$  is  $= \sqrt{\ln t} + \frac{1}{2\sqrt{\ln t}}$

- $(\ln t)^2 - \frac{1}{2(\ln t)^{1/2}}$
- $(\ln t)^2 - \frac{1}{2(\ln t)^2}$
- $(\ln t)^2 + \frac{1}{2(\ln t)^{1/2}}$

- $(\ln t)^{1/2} + \frac{1}{2(\ln t)^{1/2}}$
- $(\ln t)^{1/2} + \frac{1}{2(\ln t)^2}$

~~10~~  $10x^{-1} \rightarrow -10x^{-2}$

If  $y = \ln \frac{10}{x}$ , then  $y'$  is

$y' = \frac{1}{\frac{10}{x}} \cdot \frac{-10}{x^2} = \frac{-10}{x^2 \cdot \frac{10}{x}} = \frac{-1}{x}$

- $\ln x$
- $\frac{1}{10x}$
- $\frac{10}{x}$
- $-\frac{1}{x}$
- $\frac{1}{x}$

~~$\frac{dy}{dx} = \frac{1}{y}$~~

$\ln y = (1-x) \ln x$

$\frac{dy}{dx} \frac{1}{y} = \frac{1-x}{x} - \ln x$

$\frac{dy}{dx} = x^{-x} \left( \frac{1-x}{x} - \ln x \right)$

$= x^{-x} \left( \frac{1}{x} - 1 - \ln x \right)$

If  $f(x) = x^{1-x}$ , then  $f'(x)$  is  ~~$x^{-x}(-x)(1)$~~

- ~~$x^{1-x} \left( -\ln x + 1 - \frac{1}{x} \right)$~~
- ~~$x^{1-x} \left( -\ln x - 1 - \frac{1}{x} \right)$~~
- ~~$x^{1-x} \left( \ln x + 1 + \frac{1}{x} \right)$~~
- $x^{1-x} \left( -\ln x - 1 + \frac{1}{x} \right)$
- ~~$x^{1-x} \left( \ln x - 1 + \frac{1}{x} \right)$~~

If  $f(x) = e^{3x-1}$ , then  $f'(x)$  is  $3e^{3x-1}$

- $-\frac{1}{3}e^{3x-1}$

- $(3x - 1)e^{3x-2}$
- $\frac{1}{3}e^{3x-1}$
- $e^{3x-1}$
- $3e^{3x-1}$

If  $f(x) = \frac{1-x}{e^x}$ , then  $f'(x)$  is  $\frac{-e^x - (1-x)e^x}{e^{2x}} = \frac{-2e^x + xe^x}{e^{2x}}$

- $\frac{x-2}{e^x}$
- $\frac{1-x}{e^x}$
- $\frac{x+1}{e^x}$
- $\frac{x-1}{e^x}$
- $\frac{x+2}{e^x}$

$= \frac{-2+x}{e^x}$

If  $f(x) = e^{\sqrt{x}} + e^{-\sqrt{x}}$ , then  $f'(x)$  is

- $\frac{e^{\sqrt{x}} - e^{-\sqrt{x}}}{2\sqrt{x}}$
- $\frac{e^{\sqrt{x}} + e^{-\sqrt{x}}}{\sqrt{x}}$
- $\frac{e^{\sqrt{x}} - e^{-\sqrt{x}}}{\sqrt{x}}$
- $-\frac{e^{\sqrt{x}} + e^{-\sqrt{x}}}{2\sqrt{x}}$
- $\frac{e^{\sqrt{x}} + e^{-\sqrt{x}}}{2\sqrt{x}}$

$\frac{e^{\sqrt{x}}}{2\sqrt{x}} - \frac{e^{-\sqrt{x}}}{2\sqrt{x}}$

~~$-x^{0.5}$~~   
 $-x \rightarrow \frac{-x^{-0.5}}{2}$

If  $f(x) = \sin(2e^x)$ , then  $f'(x)$  is

$2e^x \cos 2e^x$



- $2e^x \cos(2e^x)$
- $2e^x \sin(2e^x - 1)$
- $-e^x \cos(2e^x)$
- $e^x \cos(2e^x)$
- $-2e^x \cos(2e^x)$

$y = 3^{-5x}$   
 $\ln y = -5x \ln 3$   
 $\frac{dy}{dx} \cdot \frac{1}{y} = -5 \ln 3$   
 $\frac{dy}{dx} = 3^{-5x} \cdot -5 \ln 3$

If  $f(x) = x(3^{-5x})$ , then  $f'(x)$  is  $3^{-5x} + x(3^{-5x})'(-5 \ln 3)$   
 $= 3^{-5x}(1 - 5x \ln 3)$

- $3^{-5x}(1 - 5x \ln 3)$
- $3^{-5x}(x - 5 \ln 3)$
- $x3^{-5x}(1 + 5x \ln 3)$
- $x3^{-5x}(1 - 5x \ln 3)$
- $3^{-5x}(1 + 5x \ln 3)$

RESULT

Powered by Valery Gromov



# TEST!

Test yourself!

## MAIN MENU

- Home
- Teaching
- Calculus Website
- Precalculus Website
- Tests**
  - Calculus Tests
  - Precalculus Tests

## Test

**Test:** Calculus I - Section 3.7 - Indeterminate Forms and L'Hospital's Rule - Average - Quiz 1  
**Number of Questions:** 8  
**Time:** 24 : 59

$$\lim_{\theta \rightarrow 0} \frac{\tan \theta}{\theta} = \frac{\sec^2 \theta}{1} = \frac{1}{\cos^2 \theta} = 1$$

*L'Hopital!*

- $\infty$
- 0
- $\frac{1}{2}$
- 1
- 2

$$\lim_{x \rightarrow \infty} \frac{x^{100}}{e^x} = \frac{100x^{99}}{e^x} = \dots = \frac{100!}{e^x}$$

*L'Hopital*

- $\infty$
- 1
- e
- 0
- $\frac{1}{e}$

$$\lim_{x \rightarrow 0} \frac{\sin^{-1} 2x}{x} = \frac{2 \cdot \frac{1}{\sqrt{1-x^2}}}{1} = \frac{1}{2}$$

- $\infty$
- 2
- 1

- 0
- $\frac{1}{2}$
- $\frac{2}{3}$

$$\frac{\cos 5x}{\cos 3x} = \frac{\cos 45^\circ}{\cos 27^\circ} = \frac{\cos 90^\circ}{\cos 27^\circ} = \frac{+0}{-0}$$

$$\frac{5 \sin 90^\circ}{3 \sin 270^\circ} = \frac{5}{-3} = -\frac{5}{3}$$

$\frac{\pi}{2} = 90^\circ$

$$\lim_{x \rightarrow \pi/2^-} \sec 3x \cos 5x$$

$$\frac{\cos 5x}{\cos 3x} = \frac{\cos 45^\circ}{\cos 27^\circ} = \frac{\cos 90^\circ}{\cos 27^\circ} = \frac{+0}{-0}$$

- $-\frac{5}{3}$
- $-\infty$
- $-\frac{\sqrt{2}}{2}$
- $-\frac{1}{2}$
- 0

$$y = \ln y = b \ln \left(1 + \frac{a}{x}\right)$$

$$\frac{dy}{dx} = \frac{1}{y} = \frac{1}{b \ln \left(1 + \frac{a}{x}\right)}$$

$$\frac{dy}{dx} = \frac{1}{b \ln \left(1 + \frac{a}{x}\right)} \cdot \frac{1}{1 + \frac{a}{x}} \cdot \left(-\frac{a}{x^2}\right)$$

$$x^{-1} \rightarrow -x^{-2}$$

$$\frac{1}{x} \rightarrow -\frac{1}{x^2}$$

$$\lim_{x \rightarrow \infty} (1 + a/x)^{bx}$$

- $\infty$
- $e^{ab}$
- 0
- $e^{\frac{a}{b}}$
- $e^{-\frac{a}{b}}$

$$\ln y = bx \ln \left(1 + \frac{a}{x}\right)$$

$$\frac{dy}{dx} = \left(1 + \frac{a}{x}\right)^{bx} \cdot \left(b \ln \left(1 + \frac{a}{x}\right) + \frac{bx}{1 + \frac{a}{x}} \cdot \left(-\frac{1}{x^2}\right)\right)$$

$$= \frac{1}{\left(1 + \frac{a}{x}\right)^{bx}} \cdot \frac{bx}{1 + \frac{a}{x}} \cdot \left(-\frac{1}{x^2}\right)$$

$$= \frac{a}{\left(1 + \frac{a}{x}\right)^{bx}} \cdot \frac{bx}{1 + \frac{a}{x}} = \frac{ab}{1 + \frac{a}{x}} = ab$$

$$\ln y = cb$$

$$e^{cb} = y$$

$$\lim_{x \rightarrow 1} (2-x)^{\tan(\pi/2)x}$$

- $\infty$
- 0
- e
- $e^\pi$
- $e^{\frac{2}{\pi}}$

$$\ln y = \tan \frac{\pi}{2} x \ln(2-x)$$

$$= \frac{\ln(2-x)}{\cot \frac{\pi}{2} x} \rightarrow \frac{-\frac{1}{2-x}}{\left(\frac{\pi}{2} - \cos^2 \frac{\pi}{2} x\right)}$$

$$\frac{1}{\frac{\pi}{2}} = \frac{2}{\pi}$$

$$\ln y = \frac{2}{\pi}$$

$$e^{\frac{2}{\pi}} = y$$

$$\lim_{x \rightarrow 0} (\csc x - 1/x)$$

$\infty$   
  $\frac{1}{2}$   
  $0$   
  $2$   
  $1$

$\frac{1}{\sin x} - \frac{1}{x} = \frac{x - \sin x}{x \sin x}$   
 (hopital)  $\frac{1 - \cos x}{\sin x + x \cos x} = \frac{1}{\sin x + x \cos x} - \frac{\cos x}{\sin x + x \cos x}$   
 $f'(0) = \frac{0}{0 + \infty} = 0$   
 $\frac{\sin x (\sin x + x \cos x)}{(\sin x + x \cos x)^2} = \frac{(1 - \cos x) (\cos x - \sin x + \cos x - x \sin x)}{(\sin x + x \cos x)^2}$

$= \frac{\sin x}{\cos x + \cos x - x \sin x}$   
 $= \frac{\sin x}{2 \cos x - x \sin x}$   
 $= \frac{0}{2 - 0} = 0$

$\lim_{r \rightarrow \infty} \frac{\ln(\ln r)}{\sqrt{r}}$   
 $\frac{\frac{1}{h} \cdot \frac{1}{x}}{\frac{1}{2\sqrt{x}}} = \frac{1}{x \ln x} \cdot \frac{2\sqrt{x}}{1} = \frac{2}{\sqrt{x} \ln x} = 0$

- $\infty$   
  $1$   
  $0$   
  $\sqrt{e}$   
  $e$

RESULT

Powered by Valery Gromov

$\frac{\sin^2 x + x \sin x \cos x + (\cos x - 1)(2 \cos x - x \sin x)}{(\sin x + x \cos x)^2} = \frac{\sin^2 x + 2x \cos x + x^2 \cos^2 x}{(\sin x + x \cos x)^2}$

$y''(0) = 0 + 0 + 0$

$\frac{\sin^2 x + x \sin x \cos x + 2 \cos^2 x - 2 \cos x + x \sin x - x \cos x \sin x}{(\sin x + x \cos x)^2}$

$= \frac{1 + \cos^2 x - 2 \cos x + x \sin x - x \cos x \sin x}{\sin x + x \cos x}$



# TEST!

Test yourself!

## MAIN MENU

- Home
- Teaching
- Calculus Website
- Precalculus Website
- Tests**
- Calculus Tests
- Precalculus Tests

## Test

**Test:** Calculus II - Integration Quiz 01  
**Number of Questions:** 10  
**Time:** 59 : 59

$$\int_{-2}^0 (2x + 5) dx$$

$$x^2 + 5x \Big|_{-2}^0$$

$$= -(4 - 10)$$

$$= 6$$

- 4
- 5
- 6
- 7
- 8

$$\int_0^{\pi} \sin x dx$$

$$-\cos x \Big|_0^{\pi}$$

$$= -(-1) - (-1) = 1 + 1 = 2$$

- 1
- 0
- 1
- 2
- 3

$$\int_0^{\pi} \frac{1}{2} (\cos x + |\cos x|) dx$$

$$= \frac{1}{2} (\int_0^{\pi/2} \cos x + \int_{\pi/2}^{\pi} |\cos x|)$$

$$= \frac{1}{2} (-\sin x \Big|_0^{\pi/2} + -\sin x \Big|_{\pi/2}^{\pi} + \sin x \Big|_{\pi/2}^{\pi})$$

$$= \frac{1}{2} (0 - 1 + (-1)) = (-2) \left(\frac{1}{2}\right) = -1$$

- 1
- 1
- 0
- 1/2
- 1/2

$$\int \frac{9r^2 dr}{\sqrt{1-r^3}}$$

$$(1-r^3)^{\frac{1}{2}} \rightarrow \frac{-3r^2}{2(1-r^3)^{\frac{1}{2}}} \cdot x^{-2 \cdot 3} = \frac{9r^2}{(1-r^3)^{\frac{3}{2}}}$$

$$= \frac{9r^2}{(1-r^3)^{\frac{3}{2}}} \rightarrow -6$$

- $-2(1-r^3)^{1/2} + C$
- $2(1-r^3)^{1/2} + C$
- $-6(1-r^3)^{1/2} + C$
- $-(1-r^3)^{1/2} + C$
- $(1-r^3)^{1/2} + C$

$$x^3 \rightarrow 3x^2$$

$$2\sqrt{5} \rightarrow \frac{2}{\sqrt{5}} \cdot \frac{1}{2} = \frac{1}{\sqrt{5}}$$

$$\int \frac{dx}{\sqrt{5x+8}} \quad \frac{1}{\sqrt{5}} \rightarrow 2\sqrt{5} \cdot \frac{2\sqrt{5x+8}}{5}$$

- $\frac{8}{5} \sqrt{5x+8} + C$
- $\frac{4}{5} \sqrt{5x+8} + C$
- $\frac{2}{5} \sqrt{5x+8} + C$
- $\frac{1}{5} \sqrt{5x+8} + C$
- $\frac{1}{5} \sqrt{5x+8} + C$

$$\int \tan^7\left(\frac{x}{2}\right) \sec^2\left(\frac{x}{2}\right) dx$$

$g = 2 \tan \frac{x}{2}$   
 $g' = \frac{1}{2} \sec^2 \frac{x}{2}$

$$= 2 \tan^6 \frac{x}{2} \cdot \frac{1}{2} \sec^2 \frac{x}{2} = \int \tan^6 \frac{x}{2} \cdot 2 \tan \frac{x}{2} \sec^2 \frac{x}{2} dx$$

- $\frac{1}{4} \tan^8\left(\frac{x}{2}\right) + C$
- $\frac{1}{4} \sec^8\left(\frac{x}{2}\right) + C$
- $\frac{1}{4} \cot^8\left(\frac{x}{2}\right) + C$
- $\frac{1}{4} \csc^8\left(\frac{x}{2}\right) + C$

$$= 2 \tan^8 \frac{x}{2} - \int 7 \tan^7 \frac{x}{2} \sec^2 \frac{x}{2} dx$$

$$= 2 \tan^8 \frac{x}{2} - \frac{7 \tan^6 \frac{x}{2}}{6} + C$$

$$= \frac{\tan^8 \frac{x}{2}}{4} + C$$



$\frac{1}{4} \sin^8\left(\frac{x}{2}\right) + C$

$\int x e^{2x} dx$       $\int f g' = f g - \int f' g$ ;  $f = x$   $g = \frac{e^{2x}}{2}$   $f' = 1$   $g' = e^{2x}$

$\frac{1}{2} x e^{2x} - \frac{1}{4} e^{2x} + C = \frac{x e^{2x}}{2} - \frac{e^{2x}}{4}$

$\frac{1}{2} x e^{2x} + \frac{1}{4} e^{2x} + C$

~~$-\frac{1}{2} x e^{2x} - \frac{1}{4} e^{2x} + C$~~

~~$-\frac{1}{2} x e^{2x} + \frac{1}{4} e^{2x} + C$~~

~~$-\frac{1}{2} x e^{2x} + \frac{1}{2} e^{2x} + C$~~

$(x-1)(x+1) = x^2 - 1$   
 $x-1 + \frac{1}{x+1}$   
 $= \frac{x^2 - 1 + 1}{x+1} = \frac{x^2}{x+1}$

$\int \frac{x^2}{x+1} dx$       $g' = \frac{1}{x+1}$   $g = \ln|x+1|$   $f = x^2$   $f' = 2x$       $\int \frac{x^2}{x+1} dx = x^2 \ln|x+1| - \int 2x \ln|x+1| dx + C$

$\frac{1}{2} x^2 + x - \ln|x+1| + C$       $= \int x^2 - 1 + \frac{1}{x+1}$

$-\frac{1}{2} x^2 - x + \ln|x+1| + C$       $= \frac{x^2}{2} - x + \ln|x+1|$

$\frac{1}{2} x^2 + x + \ln|x+1| + C$

$\frac{1}{2} x^2 - x - \ln|x+1| + C$

$\frac{1}{2} x^2 - x + \ln|x+1| + C$

$\int \frac{1}{\sqrt{4-x^2}} = \sin^{-1} \frac{x}{2} + C$

$\int \frac{1}{\sqrt{16-x^2}} dx = \int \frac{1}{4 \sin \theta} = \int \frac{1}{4} \csc \theta = \sin^{-1} \frac{x}{4}$

$\arctan\left(\frac{x}{4}\right) + C$

- $\arccos\left(\frac{x}{4}\right) + C$
- $\frac{1}{4} \arccos\left(\frac{x}{4}\right) + C$
- $\frac{1}{4} \arcsin\left(\frac{x}{4}\right) + C$
- $\arcsin\left(\frac{x}{4}\right) + C$

$$\int x^k = \frac{x^{k+1}}{k+1} + C$$

$$\int_2^{\infty} x^{-3/2} dx$$

~~$$\frac{3x^{-5/2}}{2} \Big|_2^{\infty} = \frac{-3}{2x^{5/2}} \Big|_2^{\infty} = 0 + \frac{3}{2\sqrt{32}}$$~~

- $\infty$
- $-\infty$
- $\sqrt{5}$
- $\sqrt{3}$
- $\sqrt{2}$

~~$$\frac{x^{-1/2}}{2} \Big|_2^{\infty} = \frac{1}{2\sqrt{x}} \Big|_2^{\infty} = 0 + \frac{1}{2\sqrt{2}} = \frac{1}{2\sqrt{2}} = \frac{\sqrt{2}}{4}$$~~



Powered by Valery Gromov

$$x^{-3/2} \rightarrow \frac{x^{-1/2}}{-1/2} = \frac{-2x^{-1/2}}{1} = -2x^{-1/2} \Big|_2^{\infty} = 0 + \frac{2}{\sqrt{2}} = \sqrt{2}$$